### Exercises 4.4-1
***
Give a simple and exact expression for nj in equation (4.12) for the case in which b is a positive integer instead of an arbitrary real number.

### `Answer`
![](http://latex.codecogs.com/gif.latex? n^j = \\lceil n / b^j \\rceil )


### Exercises 4.4-2
***
Show that if ![](http://latex.codecogs.com/gif.latex? f\(n\) = \\Theta\(n^{\\log_{b}{a}}\) \\lg^k{n} ) , where k ≥ 0, then the master recurrence has solution 
Show that if ![](http://latex.codecogs.com/gif.latex? T\(n\) = \\Theta\(n^{\\log_{b}{a}}\) \\lg^{k+1}{n} ).

### `Answer`
![](http://latex.codecogs.com/gif.latex? 
g\(n\) = \\sum_{j = 0}^{\\log_{b}{n-1}} a^jf\(n/b^j\) \\\\  ~ f\(n/b^j\) = \\Theta\\Big\(\(n/b^j\)^{\\log_b{a}}\\lg^k\(n/b^j\)\\Big\) \\\\
g\(n\) = \\Theta\\Big\(\\sum_{j=0}^{\\log_b{n}-1}a^j\\big\(\\frac{n}{b^j}\\big\)^{\\log_b{a}}\\lg^k\\big\(\\frac{n}{b^j}\\big\)\\Big\) = \\Theta\(A\) \\\\
A = \\sum_{j=0}^{\\log_b{n}-1}a^j\\big\(\\frac{n}{b^j}\\big\)^{\\log_b{a}}\\lg^k\\frac{n}{b^j}
   = n^{\\log_b{a}}\\sum_{j=0}^{\\log_b{n}-1}\\Big\(\\frac{a}{b^{\\log_b{a}}}\\Big\)^j\\lg^k\\frac{n}{b^j}
   = n^{\\log_b{a}}\\sum_{j=0}^{\\log_b{n}-1}\\lg^k\\frac{n}{b^j} 
   = n^{\\log_b{a}}B \\\\
\\lg^k\\frac{n}{d} = \(\\lg{n} - \\lg{d}\)^k = \\lg^k{n} + o\(\\lg^k{n}\) \\\\
B = \\sum_{j=0}^{\\log_b{n}-1}\\lg^k\\frac{n}{b^j}
     = \\sum_{j=0}^{\\log_b{n}-1}\\Big\(\\lg^k{n} - o\(\\lg^k{n}\)\\Big\)
     = \\log_b{n}\\lg^k{n} + \\log_b{n} \\cdot o\(\\lg^k{n}\)
     = \\Theta\(\\log_b{n}\\lg^k{n}\)
     = \\Theta\(\\lg^{k+1}{n}\) \\\\
g\(n\) = \\Theta\(A\) = \\Theta\(n^{\\log_b{a}}B\) = \\Theta\(n^{\\log_b{a}}\\lg^{k+1}{n}\)
)


### Exercises 4.3-3
***
Show that case 3 of the master theorem is overstated, in the sense that the regularity condition af(n/b) ≤ cf(n) for some constant c < 1 implies that there exists a constant ![](http://latex.codecogs.com/gif.latex? \\epsilon > 0 ~ such ~ that ~ f\(n\) = \\Omega\(n^{\\log_b{a+\\epsilon}}\)). 
### `Answer`
根据case3,我们有![](http://latex.codecogs.com/gif.latex? af\(n/b\) \\le cf\(n\) ~~~~ a \\ge 1,b \\ge 1 c < 1 )

变形一下

![](http://latex.codecogs.com/gif.latex? f\(bn\) \\ge kf\(n\) ~~~where ~ k = a/c > a \\\\ \\Rightarrow f\(b^i\) \\ge k^i f\(1\) \\\\
if~~ n = b^i, i = \\log_b{n}, then f\(n\) \\ge k^{\\log_b{n}}f\(1\) \\\\
k^{\\log_b{n}} = n^{\\log_b{k}} ~ and ~ \\log_b{k} \\ge \\log_b{a} ~so~ \\log_b{k} = \\log_b{a} + \\epsilon
)

***
Follow [@louis1992](https://github.com/gzc) on github to help finish this task.

